examples/ind_cca2.v
@@ -1,0 +1,712 @@
+From stdpp Require Import base gmap.
+From mathcomp Require Import ssreflect.
+From iris.algebra Require Import agree auth csum gset gmap excl frac.
+From iris.algebra Require Import reservation_map.
+From iris.heap_lang Require Import notation proofmode adequacy.
+From iris.heap_lang.lib Require Import par nondet_bool.
+From cryptis Require Import lib term cryptis primitives tactics.
+From cryptis Require Import role.
+From cryptis.primitives Require Import attacker.
+
+From reloc Require Import reloc.
+From cryptis Require Import lib_spec.
+From cryptis.core Require Import minted_spec term_meta_spec rel rel_inv_updates.
+From cryptis.primitives Require Import simple_spec comp_spec with_cryptis_spec.
+From cryptis.primitives Require Import attacker_spec.
+From cryptis Require Import rel_adequacy.
+From cryptis.examples Require Import ind_cpa.
+
+Set Implicit Arguments.
+Unset Strict Implicit.
+Unset Printing Implicit Defensive.
+
+Notation ind_cca2N := (nroot.@"ind_cca2").
+Notation chalN := (ind_cca2N.@"chal").
+Notation storeN := (ind_cca2N.@"store").
+Notation cellN := (ind_cca2N.@"cell").
+Notation tokenN := (ind_cca2N.@"token").
+
+Section CCA2.
+
+Context `{!relocG Σ, !public_relGS Σ}.
+Notation iProp := (iProp Σ).
+
+Implicit Types (t u : term).
+Implicit Types (skA : aenc_key).
+
+Variable N : namespace.
+
+(*
+
+A --> *: pkA
+* --> A: msg_0
+* --> A: msg_1
+A --> *: {nonce, msg_b}@pkA
+* --> A: guess
+
+The oracle answers every query t with the payload of t under skA, except
+for the challenge ciphertext.
+
+*)
+
+Definition cca_pred : seal_pred_input → seal_pred_input → iProp := λ s s',
+  match s, s' with
+  | Some (sk, pl), Some (_, pl') =>
+    ∃ seed, ⌜sk = TKey ADec seed⌝ ∧ term_meta seed chalN (pl, pl')
+  | _, _ => False
+  end%I.
+
+#[global] Instance cca_pred_persistent s s' : Persistent (cca_pred s s').
+Proof. case: s => [[??]|]; case: s' => [[??]|]; apply _. Qed.
+
+#[global] Instance cca_pred_timeless s s' : Timeless (cca_pred s s').
+Proof. case: s => [[??]|]; case: s' => [[??]|]; apply _. Qed.
+
+Definition oracle : val := rec: "loop" "c" "sk" "chal" :=
+  let: "t" := recv "c" in
+  (match: open "sk" "t" with
+     SOME "u" =>
+       if: (match: !"chal" with SOME "ct" => eq_term "ct" "t" | NONE => #false end)
+       then send "c" (TInt 0) else send "c" "u"
+   | NONE => send "c" (TInt 0)
+   end);;
+  "loop" "c" "sk" "chal".
+
+Definition alice (b : bool) : val := λ: "c",
+  let: "skA" := mk_aenc_key #() in
+  let: "pkA" := pkey "skA" in
+  let: "chal" := ref NONE in
+  Fork (oracle "c" "skA" "chal");;
+  send "c" "pkA";;
+  let: "msg_0" := recv "c" in
+  let: "msg_1" := recv "c" in
+  let: "msg" := if: #b then "msg_0" else "msg_1" in
+  let: "ct" := aenc' N "pkA" "msg" in
+  "chal" <- SOME "ct";;
+  send "c" "ct";;
+  let: "guess" := recv "c" in
+  eq_term (TInt 1) "guess".
+
+Definition alice_guess_wrapped : val := λ: "c",
+  let: "b" := nondet_bool #() in
+  ("b", if: "b" then alice true "c" else alice false "c").
+
+Definition cell_inv skA skA' (l l' : loc) : iProp :=
+  (l ↦ NONEV ∗ l' ↦ₛ NONEV ∗ term_token (seed_of_aenc_key skA) (↑chalN)) ∨
+  (∃ pl pl',
+    l ↦ SOMEV (Spec.enc (Spec.pkey skA) (Tag (N.@"m")) pl) ∗
+    l' ↦ₛ SOMEV (Spec.enc (Spec.pkey skA') (Tag (N.@"m")) pl') ∗
+    term_meta (seed_of_aenc_key skA) chalN (pl, pl') ∗
+    term_meta (seed_of_aenc_key skA) storeN () ∗
+    PUB⟨Spec.enc (Spec.pkey skA) (Tag (N.@"m")) pl,
+        Spec.enc (Spec.pkey skA') (Tag (N.@"m")) pl'⟩).
+
+Lemma open_aenc_Some seed t u :
+  Spec.open (TKey ADec seed) t = Some u ↔ t = TSeal (TKey AEnc seed) u.
+Proof.
+split.
+- rewrite /Spec.open. case: t => // k u0. case: decide => // e [<-].
+  by case: k e => //= - [] //= ? [->].
+- move=> ->. by rewrite /Spec.open decide_True.
+Qed.
+
+Lemma open_aenc_key_Some skA t u :
+  Spec.open skA t = Some u ↔ t = TSeal (Spec.pkey skA) u.
+Proof. case: skA => sA. rewrite term_of_aenc_keyE. exact: open_aenc_Some. Qed.
+
+Lemma publicly_related_TSeal_aenc_l seed u t' :
+  (∀ k' u', t' ≠ TSeal k' u') →
+  PUB⟨TSeal (TKey AEnc seed) u, t'⟩ -∗
+  wf_seal_rel AENC (Some (TKey ADec seed, u)) None.
+Proof.
+case: t' => [n'|a' b'|a'|kt' s'|k' b'|s'|pt' wf' nf'] Hns /=;
+  try by iIntros "(_ & _ & [])".
+- by iIntros "(_ & _ & _ & _ & #[_ H])".
+- by case: (Hns k' b').
+- by iIntros "(_ & _ & _ & _ & _ & _ & #[_ H])".
+Qed.
+
+Lemma publicly_related_TSeal_aenc_r t seed' u' :
+  (∀ k u, t ≠ TSeal k u) →
+  PUB⟨t, TSeal (TKey AEnc seed') u'⟩ -∗
+  wf_seal_rel AENC None (Some (TKey ADec seed', u')).
+Proof.
+case: t => [n|a b|a|kt s|k b|s|pt wf nf] Hns /=;
+  try by iIntros "(_ & _ & [])".
+- by iIntros "(_ & _ & _ & _ & #[_ H])".
+- by case: (Hns k b).
+- by iIntros "(_ & _ & _ & _ & _ & _ & #[_ H])".
+Qed.
+
+Lemma wf_seal_rel_cca s s' :
+  seal_pred_rel AENC (N.@"m") cca_pred -∗
+  inv tokenN (seal_pred_rel_token_point AENC (N.@"m")) -∗
+  wf_seal_rel AENC s s' ={⊤}=∗
+  ∃ b b', ⌜seal_pred_input_untag (N.@"m") s = Some b⌝ ∗
+          ⌜seal_pred_input_untag (N.@"m") s' = Some b'⌝ ∗
+          cca_pred b b'.
+Proof.
+iIntros "#Hpred #Htok (%N' & %Φ' & %b & %b' & %Hb & %Hb' & #HΦ' & #HΦb)".
+iInv tokenN as ">Htoken".
+iDestruct (seal_pred_rel_token_point_agree with "Htoken HΦ'") as %->.
+iModIntro. iFrame "Htoken".
+iPoseProof (seal_pred_rel_agree b b' with "Hpred HΦ'") as "#e".
+iAssert (▷ cca_pred b b')%I as "#H".
+{ iNext. by iRewrite "e". }
+iMod "H" as "#H". iModIntro. iExists b, b'. by iFrame "#".
+Qed.
+
+Lemma rel_oracle_open skA skA' t t' :
+  cryptis_rel_ctx -∗
+  seal_pred_rel AENC (N.@"m") cca_pred -∗
+  inv tokenN (seal_pred_rel_token_point AENC (N.@"m")) -∗
+  PUB⟨Spec.pkey skA, Spec.pkey skA'⟩ -∗
+  publicly_linked (Spec.pkey skA) (Spec.pkey skA') -∗
+  PUB⟨t, t'⟩ ={⊤}=∗
+  ⌜Spec.open skA t = None ∧ Spec.open skA' t' = None⌝ ∨
+  ∃ u u', ⌜Spec.open skA t = Some u ∧ Spec.open skA' t' = Some u'⌝ ∗
+    (PUB⟨u, u'⟩ ∨
+     ∃ pl pl', ⌜u = Spec.tag (Tag (N.@"m")) pl ∧ u' = Spec.tag (Tag (N.@"m")) pl'⌝ ∗
+       term_meta (seed_of_aenc_key skA) chalN (pl, pl')).
+Proof.
+case: skA => sA; case: skA' => sA'.
+rewrite term_of_aenc_keyE /term_of_aenc_key_def.
+rewrite -[seed_of_aenc_key (AEncKey sA)]/sA -[seed_of_aenc_key (AEncKey sA')]/sA'.
+rewrite -[Spec.pkey (TKey ADec sA)]/(TKey AEnc sA).
+rewrite -[Spec.pkey (TKey ADec sA')]/(TKey AEnc sA').
+iIntros "#Hctx #Hpred #Htok #Hpk #[Hlink_l Hlink_r] #Ht".
+have Hsh : ∀ t0, (∃ k u, t0 = TSeal k u) ∨ (∀ k u, t0 ≠ TSeal k u).
+{ case=> *; try by right. left; eauto. }
+case eL: (Spec.open (TKey ADec sA) t) => [u|];
+case eR: (Spec.open (TKey ADec sA') t') => [u'|].
+- move/open_aenc_Some: (eL) => ?; subst t.
+  move/open_aenc_Some: (eR) => ?; subst t'.
+  iDestruct (publicly_related_TSeal with "Ht") as "[[_ Hu]|(_ & _ & _ & _ & _ & #Hbox)]".
+  { iModIntro. iRight. iExists u, u'. iSplit; first by iPureIntro; split. by iLeft. }
+  iSimpl in "Hbox". iDestruct "Hbox" as "(_ & _ & Hwf)".
+  iMod (wf_seal_rel_cca with "Hpred Htok Hwf") as (b b') "(%Hb & %Hb' & Hcca)".
+  case/seal_pred_input_untag_Some: Hb => pl [? ?]; subst b u.
+  case/seal_pred_input_untag_Some: Hb' => pl' [? ?]; subst b' u'.
+  iSimpl in "Hcca". iDestruct "Hcca" as (seed [= <-]) "Hmeta".
+  iModIntro. iRight. iExists _, _. iSplit; first by iPureIntro; split.
+  iRight. iExists pl, pl'. by iFrame.
+- move/open_aenc_Some: (eL) => ?; subst t.
+  case: (Hsh t') => [[k' [u' ?]]|Hns]; first subst t'.
+  + iDestruct (publicly_related_TSeal with "Ht") as "[[Hk _]|(_ & _ & _ & [Hkl _] & _ & _)]".
+    * iMod (publicly_related_part_bij' with "Hctx Hpk Hk") as %Hiff; first solve_ndisj.
+      have ? : k' = TKey AEnc sA' by symmetry; apply Hiff. subst k'.
+      have := proj2 (open_aenc_Some sA' (TSeal (TKey AEnc sA') u') u') eq_refl.
+      by rewrite eR.
+    * iDestruct (linked_in_l_publicly_linked_in_l with "Hkl Hlink_l") as %?. subst k'.
+      have := proj2 (open_aenc_Some sA' (TSeal (TKey AEnc sA') u') u') eq_refl.
+      by rewrite eR.
+  + iPoseProof (publicly_related_TSeal_aenc_l _ _ Hns with "Ht") as "Hwf".
+    iMod (wf_seal_rel_cca with "Hpred Htok Hwf") as (b b') "(_ & %Hb' & Hcca)".
+    move/seal_pred_input_untag_None: Hb' => ?; subst b'.
+    case: b => [[??]|]; iSimpl in "Hcca"; by iDestruct "Hcca" as "[]".
+- move/open_aenc_Some: (eR) => ?; subst t'.
+  case: (Hsh t) => [[k [u ?]]|Hns]; first subst t.
+  + iDestruct (publicly_related_TSeal with "Ht") as "[[Hk _]|(_ & _ & _ & [_ Hkr] & _ & _)]".
+    * iMod (publicly_related_part_bij' with "Hctx Hk Hpk") as %Hiff; first solve_ndisj.
+      have ? : k = TKey AEnc sA by apply Hiff. subst k.
+      have := proj2 (open_aenc_Some sA (TSeal (TKey AEnc sA) u) u) eq_refl.
+      by rewrite eL.
+    * iDestruct (linked_in_r_publicly_linked_in_r with "Hkr Hlink_r") as %?. subst k.
+      have := proj2 (open_aenc_Some sA (TSeal (TKey AEnc sA) u) u) eq_refl.
+      by rewrite eL.
+  + iPoseProof (publicly_related_TSeal_aenc_r _ _ Hns with "Ht") as "Hwf".
+    iMod (wf_seal_rel_cca with "Hpred Htok Hwf") as (b b') "(%Hb & _ & Hcca)".
+    move/seal_pred_input_untag_None: Hb => ?; subst b.
+    iSimpl in "Hcca". by iDestruct "Hcca" as "[]".
+- iModIntro. iLeft. by iPureIntro; split.
+Qed.
+
+Lemma rel_send_fail c c' :
+  channel_rel c c' -∗
+  REL send c (TInt 0) << send c' (TInt 0) : lrel_unit.
+Proof.
+iIntros "#Hc". iApply (rel_send with "Hc"). iNext. by rewrite publicly_related_TInt.
+Qed.
+
+Lemma rel_oracle c c' skA skA' (l l' : loc) :
+  cryptis_rel_ctx -∗
+  seal_pred_rel AENC (N.@"m") cca_pred -∗
+  inv tokenN (seal_pred_rel_token_point AENC (N.@"m")) -∗
+  inv cellN (cell_inv skA skA' l l') -∗
+  channel_rel c c' -∗
+  PUB⟨Spec.pkey skA, Spec.pkey skA'⟩ -∗
+  publicly_linked (Spec.pkey skA) (Spec.pkey skA') -∗
+  REL oracle c skA #l << oracle c' skA' #l' : lrel_unit.
+Proof.
+iIntros "#Hctx #Hpred #Htok #Hcell #Hc #Hpk #Hlink".
+iLöb as "IH".
+rel_rec_l. rel_rec_r. rel_pures_l. rel_pures_r.
+rel_bind_l (recv _). rel_bind_r (recv _).
+iApply refines_bind'. iApply rel_recv=> //.
+iIntros (t t') "#Ht"=> /=.
+rel_pures_l. rel_pures_r.
+rel_apply_l rel_open_l. rel_apply_r rel_open_r.
+iMod (rel_oracle_open with "Hctx Hpred Htok Hpk Hlink Ht")
+  as "[[-> ->]|(%u & %u' & [%eL %eR] & #Hu)]".
+- rel_pures_l. rel_pures_r.
+  rel_bind_l (send _ _). rel_bind_r (send _ _).
+  iApply refines_bind; first by iApply rel_send_fail.
+  iIntros (? ?) "[-> ->]"=> /=.
+  rel_pures_l. rel_pures_r. by iApply "IH".
+- rewrite eL eR. rel_pures_l. rel_pures_r.
+  rel_load_l_atomic.
+  iInv cellN as "[(Hl & Hl' & >Htoken)|(%pl & %pl' & Hl & Hl' & >#Hmeta & >#Hstore & #Hct)]" "Hclose".
+  + iDestruct "Hu" as "[#Hu|(%pl & %pl' & _ & #Hmeta)]"; last first.
+    { by iDestruct (term_meta_token with "Htoken Hmeta") as "[]". }
+    iModIntro. iExists _. iFrame "Hl". iIntros "!> Hl".
+    rel_load_r.
+    iMod ("Hclose" with "[Hl Hl' Htoken]") as "_".
+    { iNext. iLeft. iFrame. }
+    rel_pures_l. rel_pures_r.
+    rel_bind_l (send _ _). rel_bind_r (send _ _).
+    iApply refines_bind; first by iApply rel_send.
+    iIntros (? ?) "[-> ->]"=> /=.
+    rel_pures_l. rel_pures_r. by iApply "IH".
+  + iModIntro. iExists _. iFrame "Hl". iIntros "!> Hl".
+    rel_load_r.
+    iMod ("Hclose" with "[Hl Hl']") as "_".
+    { iNext. iRight. iExists pl, pl'. by iFrame "#∗". }
+    rel_pures_l. rel_pures_r.
+    rel_apply_l rel_eq_term_l. rel_apply_r rel_eq_term_r.
+    set ct := Spec.enc (Spec.pkey skA) (Tag (N.@"m")) pl.
+    set ct' := Spec.enc (Spec.pkey skA') (Tag (N.@"m")) pl'.
+    iMod (publicly_related_part_bij' ct ct' t t' ltac:(solve_ndisj)
+            with "Hctx Hct Ht") as %Hiff.
+    iAssert (⌜ct = t⌝ ∨ (⌜ct ≠ t⌝ ∗ PUB⟨u, u'⟩))%I as "[%e|[%ne #Hu']]".
+    { iDestruct "Hu" as "[#Hu|(%pl1 & %pl1' & [-> ->] & #Hmeta1)]".
+      - case: (decide (ct = t)) => [e|ne]; first by iLeft.
+        iRight. by iSplit.
+      - iDestruct (term_meta_agree with "Hmeta Hmeta1") as %[= <- <-].
+        iLeft. iPureIntro. move/open_aenc_key_Some: eL => ->.
+        by rewrite /ct /Spec.enc. }
+    * have e' : ct' = t' by apply Hiff.
+      rewrite !bool_decide_eq_true_2 //.
+      rel_pures_l. rel_pures_r.
+      rel_bind_l (send _ _). rel_bind_r (send _ _).
+      iApply refines_bind; first by iApply rel_send_fail.
+      iIntros (? ?) "[-> ->]"=> /=.
+      rel_pures_l. rel_pures_r. by iApply "IH".
+    * have ne' : ct' ≠ t' by rewrite -Hiff.
+      rewrite !bool_decide_eq_false_2 //.
+      rel_pures_l. rel_pures_r.
+      rel_bind_l (send _ _). rel_bind_r (send _ _).
+      iApply refines_bind; first by iApply rel_send.
+      iIntros (? ?) "[-> ->]"=> /=.
+      rel_pures_l. rel_pures_r. by iApply "IH".
+Qed.
+
+Lemma rel_aenc' (skA skA' : aenc_key) (m m' : term) (Ψ : val → val → iProp) :
+  cryptis_rel_ctx -∗
+  seal_pred_rel AENC (N.@"m") cca_pred -∗
+  ⌜is_nonce (seed_of_aenc_key skA)⌝ -∗
+  minted (Spec.pkey skA) -∗
+  minted_spec (Spec.pkey skA') -∗
+  publicly_linked (Spec.pkey skA) (Spec.pkey skA') -∗
+  secret_in_l (seed_of_aenc_key skA) -∗
+  minted m -∗ minted_spec m' -∗
+  (∀ pl pl',
+    (∀ E, ⌜↑cryptisN ⊆ E⌝ -∗
+      cca_pred (Some (skA : term, pl)) (Some (skA' : term, pl')) ={E}=∗
+      PUB⟨Spec.enc (Spec.pkey skA) (Tag (N.@"m")) pl,
+          Spec.enc (Spec.pkey skA') (Tag (N.@"m")) pl'⟩) ={⊤}=∗
+    Ψ (Spec.enc (Spec.pkey skA) (Tag (N.@"m")) pl)
+      (Spec.enc (Spec.pkey skA') (Tag (N.@"m")) pl')) -∗
+  REL aenc' N (Spec.pkey skA) m
+   << aenc' N (Spec.pkey skA') m' : Ψ.
+Proof.
+iIntros "#Hctx #Hpred %Hnonce_a #mint_pk #mint_spec_pk' #elem_pk #secret_a #mint_m #mint_spec_m' post".
+rewrite /aenc'.
+rel_pures_l. rel_pures_r.
+rel_apply_l (rel_mk_nonce_l _ _
+  (λ n, {[ n;
+           Spec.of_list [n; m];
+           Spec.tag (Tag (N.@"m")) (Spec.of_list [n; m]);
+           Spec.enc (Spec.pkey skA) (Tag (N.@"m")) (Spec.of_list [n; m]) ]})
+  with "[//]").
+{ iIntros "%t". rewrite big_sepS_forall. iIntros (t' Ht').
+  rewrite !elem_of_union !elem_of_singleton in Ht'.
+  case: Ht' => [[[->|->]|->]|->]; iModIntro.
+  - by iSplit; iIntros "?".
+  - rewrite minted_of_list /=. iSplit; iIntros "#H".
+    + by iFrame "#".
+    + by iDestruct "H" as "[? _]".
+  - rewrite minted_tag minted_of_list /=. iSplit; iIntros "#H".
+    + by iFrame "#".
+    + by iDestruct "H" as "[? _]".
+  - rewrite /Spec.enc minted_TSeal minted_tag minted_of_list /=. iSplit; iIntros "#H".
+    + by iFrame "#".
+    + by iDestruct "H" as "[_ [? _]]". }
+iIntros (n) "%Hn #mint_n Htt".
+rel_apply_r (rel_mk_nonce_r _ _
+  (λ n, {[ n;
+           Spec.of_list [n; m'];
+           Spec.tag (Tag (N.@"m")) (Spec.of_list [n; m']);
+           Spec.enc (Spec.pkey skA') (Tag (N.@"m")) (Spec.of_list [n; m']) ]})
+  with "[//]").
+{ iIntros "%t". rewrite big_sepS_forall. iIntros (t' Ht').
+  rewrite !elem_of_union !elem_of_singleton in Ht'.
+  case: Ht' => [[[->|->]|->]|->]; iModIntro.
+  - by iSplit; iIntros "?".
+  - rewrite minted_spec_of_list /=. iSplit; iIntros "#H".
+    + by iFrame "#".
+    + by iDestruct "H" as "[? _]".
+  - rewrite minted_spec_tag minted_spec_of_list /=. iSplit; iIntros "#H".
+    + by iFrame "#".
+    + by iDestruct "H" as "[? _]".
+  - rewrite /Spec.enc minted_spec_TSeal minted_spec_tag minted_spec_of_list /=.
+    iSplit; iIntros "#H".
+    + by iFrame "#".
+    + by iDestruct "H" as "[_ [? _]]". }
+iIntros (n') "%Hn' #mint_spec_n' Htts".
+set pl := Spec.of_list [n; m].
+set tg := Spec.tag (Tag (N.@"m")) pl.
+set c := Spec.enc (Spec.pkey skA) (Tag (N.@"m")) pl.
+set pl' := Spec.of_list [n'; m'].
+set tg' := Spec.tag (Tag (N.@"m")) pl'.
+set c' := Spec.enc (Spec.pkey skA') (Tag (N.@"m")) pl'.
+case/is_nonceP: (Hn) => [an En]. case/is_nonceP: (Hn') => [an' En'].
+(* Split the tokens. *)
+have Hd_c : ({[n]} ∪ {[pl]} ∪ {[tg]} : gset term) ## {[c]}.
+{ rewrite /c /tg /pl /Spec.enc Spec.tag_unseal Spec.of_list_unseal En /=. set_solver. }
+have Hd_tg : ({[n]} ∪ {[pl]} : gset term) ## {[tg]}.
+{ rewrite /tg /pl Spec.tag_unseal Spec.of_list_unseal Tag_unseal En /=. set_solver. }
+have Hd_pl : ({[n]} : gset term) ## {[pl]}.
+{ rewrite /pl Spec.of_list_unseal En /=. set_solver. }
+have Hd_c' : ({[n']} ∪ {[pl']} ∪ {[tg']} : gset term) ## {[c']}.
+{ rewrite /c' /tg' /pl' /Spec.enc Spec.tag_unseal Spec.of_list_unseal En' /=. set_solver. }
+have Hd_tg' : ({[n']} ∪ {[pl']} : gset term) ## {[tg']}.
+{ rewrite /tg' /pl' Spec.tag_unseal Spec.of_list_unseal Tag_unseal En' /=. set_solver. }
+have Hd_pl' : ({[n']} : gset term) ## {[pl']}.
+{ rewrite /pl' Spec.of_list_unseal En' /=. set_solver. }
+rewrite big_sepS_union // big_sepS_union // big_sepS_union // !big_sepS_singleton.
+iDestruct "Htt" as "(((tt_n & tt_pl) & tt_tg) & tt_c)".
+rewrite big_sepS_union // big_sepS_union // big_sepS_union // !big_sepS_singleton.
+iDestruct "Htts" as "(((tts_n & tts_pl) & tts_tg) & tts_c)".
+rewrite (term_token_difference n (↑cryptisN.@"public_rel".@"flow") ⊤)=> //.
+iDestruct "tt_n" as "[tt_n_flow tt_n]".
+rewrite (term_token_difference n (↑cryptisN.@"public_rel".@"map")
+           (⊤ ∖ ↑cryptisN.@"public_rel".@"flow")); last solve_ndisj.
+iDestruct "tt_n" as "[tt_n_map _]".
+rewrite (term_token_difference pl (↑cryptisN.@"public_rel".@"flow") ⊤)=> //.
+iDestruct "tt_pl" as "[tt_pl_flow tt_pl]".
+rewrite (term_token_difference pl (↑cryptisN.@"public_rel".@"map")
+           (⊤ ∖ ↑cryptisN.@"public_rel".@"flow")); last solve_ndisj.
+iDestruct "tt_pl" as "[tt_pl_map _]".
+rewrite (term_token_difference tg (↑cryptisN.@"public_rel".@"map") ⊤)=> //.
+iDestruct "tt_tg" as "[tt_tg_map _]".
+rewrite (term_token_difference c (↑cryptisN.@"public_rel".@"flow") ⊤)=> //.
+iDestruct "tt_c" as "[tt_c_flow tt_c]".
+rewrite (term_token_difference c (↑cryptisN.@"public_rel".@"map")
+           (⊤ ∖ ↑cryptisN.@"public_rel".@"flow")); last solve_ndisj.
+iDestruct "tt_c" as "[tt_c_map _]".
+rewrite (term_token_spec_difference n' (↑cryptisN.@"public_rel".@"flow") ⊤)=> //.
+iDestruct "tts_n" as "[tts_n_flow tts_n]".
+rewrite (term_token_spec_difference n' (↑cryptisN.@"public_rel".@"map")
+           (⊤ ∖ ↑cryptisN.@"public_rel".@"flow")); last solve_ndisj.
+iDestruct "tts_n" as "[tts_n_map _]".
+rewrite (term_token_spec_difference pl' (↑cryptisN.@"public_rel".@"flow") ⊤)=> //.
+iDestruct "tts_pl" as "[tts_pl_flow tts_pl]".
+rewrite (term_token_spec_difference pl' (↑cryptisN.@"public_rel".@"map")
+           (⊤ ∖ ↑cryptisN.@"public_rel".@"flow")); last solve_ndisj.
+iDestruct "tts_pl" as "[tts_pl_map _]".
+rewrite (term_token_spec_difference tg' (↑cryptisN.@"public_rel".@"map") ⊤)=> //.
+iDestruct "tts_tg" as "[tts_tg_map _]".
+rewrite (term_token_spec_difference c' (↑cryptisN.@"public_rel".@"flow") ⊤)=> //.
+iDestruct "tts_c" as "[tts_c_flow tts_c]".
+rewrite (term_token_spec_difference c' (↑cryptisN.@"public_rel".@"map")
+           (⊤ ∖ ↑cryptisN.@"public_rel".@"flow")); last solve_ndisj.
+iDestruct "tts_c" as "[tts_c_map _]".
+(* The tagged payload is protected by the chain nonce → payload → tagged payload. *)
+have Hsub_pl : is_immediate_subterm n pl.
+{ rewrite /pl Spec.of_list_unseal /=. exact: SubtermPairL. }
+have Hsub_tg : is_immediate_subterm pl tg.
+{ rewrite /tg Spec.tag_unseal. exact: SubtermPairR. }
+have Hsub_pl' : is_immediate_subterm n' pl'.
+{ rewrite /pl' Spec.of_list_unseal /=. exact: SubtermPairL. }
+have Hsub_tg' : is_immediate_subterm pl' tg'.
+{ rewrite /tg' Spec.tag_unseal. exact: SubtermPairR. }
+iMod (public_rel_flow_l_extend (E:=⊤) n ltac:(solve_ndisj)
+        with "Hctx tt_n_flow tt_n_map") as "[prot_n tt_n_map]".
+iMod (public_rel_flow_l_grow_2 (E:=⊤) Hn ltac:(solve_ndisj) Hsub_pl
+        with "Hctx prot_n tt_n_map") as "(prot_n & protby_pl & tt_n_map)".
+iMod (public_rel_flow_l_extend (E:=⊤) pl ltac:(solve_ndisj)
+        with "Hctx tt_pl_flow tt_pl_map") as "[prot_pl tt_pl_map]".
+iMod (public_rel_flow_l_grow_3 (E:=⊤) n ltac:(solve_ndisj) Hsub_tg
+        with "Hctx protby_pl prot_pl tt_pl_map") as "(prot_pl & protby_tg & protby_pl & tt_pl_map)".
+iMod (public_rel_flow_r_extend (E:=⊤) n' ltac:(solve_ndisj)
+        with "Hctx tts_n_flow tts_n_map") as "[prot_n' tts_n_map]".
+iMod (public_rel_flow_r_grow_2 (E:=⊤) Hn' ltac:(solve_ndisj) Hsub_pl'
+        with "Hctx prot_n' tts_n_map") as "(prot_n' & protby_pl' & tts_n_map)".
+iMod (public_rel_flow_r_extend (E:=⊤) pl' ltac:(solve_ndisj)
+        with "Hctx tts_pl_flow tts_pl_map") as "[prot_pl' tts_pl_map]".
+iMod (public_rel_flow_r_grow_3 (E:=⊤) n' ltac:(solve_ndisj) Hsub_tg'
+        with "Hctx protby_pl' prot_pl' tts_pl_map") as "(prot_pl' & protby_tg' & protby_pl' & tts_pl_map)".
+iMod (linked_extend (E:=⊤) tg tg' pl pl' ltac:(solve_ndisj)
+        with "Hctx protby_tg protby_tg' tt_tg_map tts_tg_map") as "(_ & _ & #priv_tg & _ & _)".
+(* The secret keys can never become publicly related. *)
+iAssert (□ (PUB⟨skA, skA'⟩ → PUB⟨pl, pl'⟩))%I as "#Hbox".
+{ iIntros "!> #Hsk". iExFalso.
+  rewrite publicly_related_adec_key'.
+  iDestruct (publicly_related_nonce_term _ Hnonce_a with "Hsk") as "[Hl _]".
+  by iDestruct (secret_in_l_publicly_linked_in_l with "secret_a Hl") as "[]". }
+iAssert (minted pl) as "#mint_pl".
+{ rewrite /pl minted_of_list /=. by iFrame "#". }
+iAssert (minted_spec pl') as "#mint_spec_pl'".
+{ rewrite /pl' minted_spec_of_list /=. by iFrame "#". }
+iMod (public_rel_flow_l_extend (E:=⊤) c ltac:(solve_ndisj)
+        with "Hctx tt_c_flow tt_c_map") as "[prot_c tt_c_map]".
+iMod (public_rel_flow_r_extend (E:=⊤) c' ltac:(solve_ndisj)
+        with "Hctx tts_c_flow tts_c_map") as "[prot_c' tts_c_map]".
+(* The ciphertexts are linked later, once they are recorded as the challenge. *)
+iMod ("post" $! pl pl' with "[prot_c prot_c' tt_c_map tts_c_map]") as "post".
+{ iIntros (E HE) "#Hcca".
+  iAssert (□ (publicly_linked c c' -∗ PUB⟨c, c'⟩))%I as "#Hwand".
+  { iIntros "!> #elem_c". rewrite publicly_related_aenc. iRight.
+    do 5 (iSplit; first done).
+    iSplit; first by iApply publicly_linked_linked.
+    iSplit; first done. iSplit; first done.
+    iExists (N.@"m"), cca_pred, (Some (skA : term, pl)), (Some (skA' : term, pl')).
+    do 2 (iSplit; first by iPureIntro; apply seal_pred_input_untag_tag).
+    iSplit; first done. by iIntros "!> !>". }
+  iMod (public_rel_extend c c' HE
+          with "Hctx Hwand prot_c prot_c' tt_c_map tts_c_map") as "#elem_c".
+  iModIntro. by iApply "Hwand". }
+(* Run the program. *)
+rel_pures_l. rel_pures_r.
+rel_apply_l rel_nil_l.
+repeat rel_apply_l rel_cons_l. rel_apply_l rel_term_of_list_l.
+rel_apply_r rel_nil_r.
+repeat rel_apply_r rel_cons_r. rel_apply_r rel_term_of_list_r.
+rel_apply_l rel_aenc'_l. iModIntro.
+rel_apply_r rel_aenc'_r.
+by rel_values.
+Qed.
+
+Lemma rel_alice c c' (b b' : bool) :
+  cryptis_rel_ctx -∗
+  seal_pred_rel AENC (N.@"m") cca_pred -∗
+  inv tokenN (seal_pred_rel_token_point AENC (N.@"m")) -∗
+  channel_rel c c' -∗
+  REL alice b c << alice b' c' : lrel_bool.
+Proof.
+iIntros "#Hctx #Hpred #Htok #Hc". rewrite /alice.
+rel_pures_l. rel_pures_r.
+have Hdisj : ∀ sk : aenc_key,
+    seed_of_aenc_key sk ∉ (∅ : gset term) ∧
+    seed_of_aenc_key sk ∉ ({[Spec.pkey sk]} : gset term) ∧
+    (∅ : gset term) ## ({[Spec.pkey sk]} : gset term).
+{ move=> sk. rewrite /Spec.pkey [term_of_aenc_key]unlock /=.
+  have Hne : ∀ kt (t : term), t ≠ TKey kt t.
+  { move=> kt t H. have := f_equal tsize H.
+    rewrite (tsize_eq (TKey kt t)). lia. }
+  set_solver. }
+rel_apply_l (rel_mk_aenc_key_l _ _ (λ _, ∅) (λ t, {[t]}) _ Hdisj with "[//]").
+{ iIntros "%sk". by rewrite big_sepS_empty. }
+{ iIntros "%sk". rewrite big_sepS_singleton. iModIntro. by iSplit; iIntros "?". }
+iIntros (skA) "%Hnonce_a #mint_skA token_a _ token_pkA".
+rewrite big_sepS_singleton.
+rel_apply_r (rel_mk_aenc_key_r _ _ (λ _, ∅) (λ t, {[t]}) _ Hdisj with "[//]").
+{ iIntros "%sk". by rewrite big_sepS_empty. }
+{ iIntros "%sk". rewrite big_sepS_singleton. iModIntro. by iSplit; iIntros "?". }
+iIntros (skA') "%Hnonce_a' #mint_spec_skA' token_spec_a _ token_spec_pkA'".
+rewrite big_sepS_singleton.
+rel_pures_l. rel_pures_r.
+rel_apply_l rel_pkey_l. rel_apply_r rel_pkey_r.
+rel_pures_l. rel_pures_r.
+(* Tokens. *)
+rewrite (term_token_difference (seed_of_aenc_key skA) (↑cryptisN.@"public_rel".@"map") ⊤)=> //.
+iDestruct "token_a" as "[token_a token_a_rest]".
+rewrite (term_token_difference (seed_of_aenc_key skA) (↑chalN)
+           (⊤ ∖ ↑cryptisN.@"public_rel".@"map")); last solve_ndisj.
+iDestruct "token_a_rest" as "[token_chal token_a_rest]".
+rewrite (term_token_difference (seed_of_aenc_key skA) (↑storeN)
+           ((⊤ ∖ ↑cryptisN.@"public_rel".@"map") ∖ ↑chalN)); last solve_ndisj.
+iDestruct "token_a_rest" as "[token_store _]".
+rewrite (term_token_spec_difference (seed_of_aenc_key skA') (↑cryptisN.@"public_rel".@"map") ⊤)=> //.
+iDestruct "token_spec_a" as "[token_spec_a _]".
+rewrite (term_token_difference (Spec.pkey skA)
+           (↑cryptisN.@"public_rel".@"flow") ⊤)=> //.
+iDestruct "token_pkA" as "[token_pkA_flow token_pkA]".
+rewrite (term_token_difference (Spec.pkey skA)
+           (↑cryptisN.@"public_rel".@"map") (⊤ ∖ ↑cryptisN.@"public_rel".@"flow"));
+  last solve_ndisj.
+iDestruct "token_pkA" as "[token_pkA_map _]".
+rewrite (term_token_spec_difference (Spec.pkey skA')
+           (↑cryptisN.@"public_rel".@"flow") ⊤)=> //.
+iDestruct "token_spec_pkA'" as "[token_spec_pkA_flow token_spec_pkA']".
+rewrite (term_token_spec_difference (Spec.pkey skA')
+           (↑cryptisN.@"public_rel".@"map") (⊤ ∖ ↑cryptisN.@"public_rel".@"flow"));
+  last solve_ndisj.
+iDestruct "token_spec_pkA'" as "[token_spec_pkA_map _]".
+(* The seeds never become public. *)
+iMod (public_rel_secret_l_2 (E:=⊤) Hnonce_a ltac:(solve_ndisj) with "Hctx token_a") as "#secret_a".
+iMod (public_rel_secret_r_2 (E:=⊤) Hnonce_a' ltac:(solve_ndisj) with "Hctx token_spec_a") as "#secret_a'".
+(* The public keys are publicly related. *)
+iMod (public_rel_flow_l_extend (E:=⊤) (Spec.pkey skA) ltac:(solve_ndisj)
+        with "Hctx token_pkA_flow token_pkA_map") as "[prot_pkA token_pkA_map]".
+iMod (public_rel_flow_r_extend (E:=⊤) (Spec.pkey skA') ltac:(solve_ndisj)
+        with "Hctx token_spec_pkA_flow token_spec_pkA_map") as "[prot_pkA' token_spec_pkA_map]".
+iAssert (□ (publicly_linked (Spec.pkey skA) (Spec.pkey skA') -∗
+            PUB⟨Spec.pkey skA, Spec.pkey skA'⟩))%I as "#Hwand".
+{ iIntros "!> #elem". rewrite publicly_related_aenc_key. iRight.
+  do 3 (iSplit; first done).
+  iSplit; [by iApply secret_in_l_linked_in_l | by iApply secret_in_r_linked_in_r]. }
+iMod (public_rel_extend (E:=⊤) (Spec.pkey skA) (Spec.pkey skA')
+        ltac:(solve_ndisj)
+        with "Hctx Hwand prot_pkA prot_pkA' token_pkA_map token_spec_pkA_map") as "#elem_pkA".
+iPoseProof ("Hwand" with "elem_pkA") as "#Hpub".
+(* The challenge cell and the oracle. *)
+rel_alloc_l l as "Hl". rel_alloc_r l' as "Hl'".
+rel_pures_l. rel_pures_r.
+iMod (inv_alloc cellN _ (cell_inv skA skA' l l') with "[Hl Hl' token_chal]") as "#Hcell".
+{ iNext. iLeft. iFrame. }
+rel_bind_l (Fork _). rel_bind_r (Fork _).
+iApply refines_bind.
+{ iApply refines_fork.
+  iApply (rel_oracle with "Hctx Hpred Htok Hcell Hc Hpub elem_pkA"). }
+iIntros (? ?) "_" => /=.
+rel_pures_l. rel_pures_r.
+rel_bind_l (send _ _). rel_bind_r (send _ _).
+iApply refines_bind; first by iApply rel_send.
+iIntros (? ?) "[-> ->]"=> /=.
+rel_pures_l. rel_pures_r.
+rel_bind_l (recv _). rel_bind_r (recv _).
+iApply refines_bind'. iApply rel_recv=> //.
+iIntros (msg_0 msg_0') "#Hmsg_0"=> /=.
+rel_pures_l. rel_pures_r.
+rel_bind_l (recv _). rel_bind_r (recv _).
+iApply refines_bind'. iApply rel_recv=> //.
+iIntros (msg_1 msg_1') "#Hmsg_1"=> /=.
+rel_pures_l. rel_pures_r.
+rel_bind_l (if: _ then _ else _)%E.
+rel_bind_r (if: _ then _ else _)%E.
+iApply (refines_bind _ _ _ (λ v v', ∃ m m' : term, ⌜v = m⌝ ∧ ⌜v' = m'⌝ ∧ minted m ∧ minted_spec m')%I).
+{ rewrite (publicly_related_minted msg_0) (publicly_related_minted msg_1).
+  iDestruct "Hmsg_0" as "[? ?]".
+  iDestruct "Hmsg_1" as "[? ?]".
+  case: b; case: b'; rel_pures_l; rel_pures_r; rel_values.
+  - iExists msg_0, msg_0'; iFrame "#"; eauto.
+  - iExists msg_0, msg_1'; iFrame "#"; eauto.
+  - iExists msg_1, msg_0'; iFrame "#"; eauto.
+  - iExists msg_1, msg_1'; iFrame "#"; eauto. }
+iIntros (? ?) "(%msg & %msg' & -> & -> & #mint_msg & #mint_spec_msg')"=> /=.
+rel_pures_l. rel_pures_r.
+rel_bind_l (aenc' N _ _). rel_bind_r (aenc' N _ _).
+iApply (refines_bind _ _ _ (λ v v', ∃ pl pl',
+  ⌜v = Spec.enc (Spec.pkey skA) (Tag (N.@"m")) pl⌝ ∗
+  ⌜v' = Spec.enc (Spec.pkey skA') (Tag (N.@"m")) pl'⌝ ∗
+  (∀ E, ⌜↑cryptisN ⊆ E⌝ -∗
+     cca_pred (Some (skA : term, pl)) (Some (skA' : term, pl')) ={E}=∗
+     PUB⟨Spec.enc (Spec.pkey skA) (Tag (N.@"m")) pl,
+         Spec.enc (Spec.pkey skA') (Tag (N.@"m")) pl'⟩))%I).
+{ iApply (rel_aenc' skA skA' msg msg' with "Hctx Hpred [//] [] [] elem_pkA secret_a mint_msg mint_spec_msg'").
+  - by rewrite minted_pkey.
+  - by rewrite minted_spec_pkey.
+  - iIntros (pl pl') "link". iModIntro. iExists pl, pl'. by iFrame. }
+iIntros (? ?) "(%pl & %pl' & -> & -> & link)"=> /=.
+rel_pures_l. rel_pures_r.
+(* Store the challenge and link it. *)
+rel_store_l_atomic.
+iInv cellN as "[(Hl & Hl' & >token_chal)|(%pl0 & %pl0' & Hl & Hl' & _ & >#Hstore0 & _)]" "Hclose";
+  last first.
+{ by iDestruct (term_meta_token with "token_store Hstore0") as "[]". }
+iMod (term_meta_set chalN (pl, pl') (↑chalN) (seed_of_aenc_key skA) ltac:(done)
+        with "token_chal") as "#Hmeta".
+iMod (term_meta_set storeN () (↑storeN) (seed_of_aenc_key skA) ltac:(done)
+        with "token_store") as "#Hstore".
+iMod ("link" $! (⊤ ∖ ↑cellN) with "[] []") as "#Hct".
+{ iPureIntro. solve_ndisj. }
+{ iSimpl. iExists (seed_of_aenc_key skA). iSplit; last done.
+  iPureIntro. by rewrite term_of_aenc_keyE. }
+iModIntro. iExists _. iFrame "Hl". iIntros "!> Hl".
+rel_store_r.
+iMod ("Hclose" with "[Hl Hl']") as "_".
+{ iNext. iRight. iExists pl, pl'. by iFrame "#∗". }
+rel_pures_l. rel_pures_r.
+rel_bind_l (send _ _). rel_bind_r (send _ _).
+iApply refines_bind; first by iApply rel_send.
+iIntros (? ?) "[-> ->]"=> /=.
+rel_pures_l. rel_pures_r.
+rel_bind_l (recv _). rel_bind_r (recv _).
+iApply refines_bind'. iApply rel_recv=> //.
+iIntros (guess guess') "#Hguess"=> /=.
+rel_pures_l. rel_pures_r.
+rel_apply_l rel_eq_term_l. rel_apply_r rel_eq_term_r.
+rel_values.
+iMod (publicly_related_part_bij' (E:=⊤) (TInt 1) (TInt 1) guess guess'
+        ltac:(solve_ndisj)
+        with "Hctx [] Hguess") as %H.
+{ by rewrite publicly_related_TInt. }
+iModIntro. iExists (bool_decide (TInt 1 = guess)). iPureIntro.
+split; first done. do 2 f_equal. by apply bool_decide_ext.
+Qed.
+
+Lemma rel_alice_guess_wrapped c c' :
+  cryptis_rel_ctx -∗
+  seal_pred_rel AENC (N.@"m") cca_pred -∗
+  inv tokenN (seal_pred_rel_token_point AENC (N.@"m")) -∗
+  channel_rel c c' -∗
+  REL alice_guess_wrapped c << alice_guess_wrapped c' : λ p1 p2,
+    ⌜∃ b g b' g' : bool,
+    p1 = (#b, #g)%V ∧ p2 = (#b', #g')%V ∧ b' = negb b ∧ g = g'⌝.
+Proof.
+iIntros "#Hctx #Hpred #Htok #Hc". rewrite /alice_guess_wrapped.
+rel_pures_l. rel_pures_r.
+rel_apply_l rel_nondet_bool_l. iIntros (choice).
+rel_apply_r (rel_nondet_bool_r _ _ (negb choice)).
+case: choice; rel_pures_l; rel_pures_r.
+- rel_bind_l (alice true _). rel_bind_r (alice false _).
+  iApply refines_bind; first by iApply rel_alice.
+  iIntros (v v') "(%g & %e & %e')"; subst v v' => /=.
+  rel_pures_l. rel_pures_r. rel_values.
+  iPureIntro. by exists true, g, false, g.
+- rel_bind_l (alice false _). rel_bind_r (alice true _).
+  iApply refines_bind; first by iApply rel_alice.
+  iIntros (v v') "(%g & %e & %e')"; subst v v' => /=.
+  rel_pures_l. rel_pures_r. rel_values.
+  iPureIntro. by exists false, g, true, g.
+Qed.
+
+End CCA2.
+
+Definition ind_cca2_game N (b : bool) : expr :=
+  (λ: "adv", run_network_rel "adv" (alice N b))%E.
+
+(** IND-CCA2 as a contextual equivalence: no well-typed attacker with a
+    decryption oracle for every ciphertext but the challenge can tell which
+    of its two messages Alice encrypts. *)
+Theorem ind_cca2_ctx_equiv N b b' :
+  ∅ ⊨ ind_cca2_game N b =ctx= ind_cca2_game N b' : (attacker_ty → TBool)%ty.
+Proof.
+split; apply: cryptis_ctx_refinement => Σ ? ? Δ; iIntros "#Hctx Haenc _ _ _";
+  iMod (seal_pred_rel_set_point AENC (N.@"m") cca_pred with "Haenc")
+    as "[#Hpred Htoken]";
+  iMod (inv_alloc tokenN _ (seal_pred_rel_token_point AENC (N.@"m")) with "Htoken")
+    as "#Htok";
+  iIntros "!> !> %c %c' #Hc"; by iApply (rel_alice with "Hctx Hpred Htok Hc").
+Qed.
+
+(** The same fact as an adequacy statement for the nondeterministic game. *)
+Theorem ind_cca2_secure Σ `{!relocPreG Σ, !public_relGpreS Σ} N (adv : val) σ :
+  (∀ `{!relocG Σ}, ⊢ REL adv << adv : attacker_rel) →
+  adequate NotStuck (run_network_rel adv (alice_guess_wrapped N)) σ
+    (λ v _, ∃ thp' h v',
+       rtc erased_step ([run_network_rel adv (alice_guess_wrapped N)], σ)
+         (of_val v' :: thp', h) ∧
+       ∃ b g b' g' : bool,
+         v = (#b, #g)%V ∧ v' = (#b', #g')%V ∧ b' = negb b ∧ g = g').
+Proof.
+move=> Hadv. apply: cryptis_rel_adequacy => // ? ?.
+iIntros "#Hctx Haenc _ _ _".
+iMod (seal_pred_rel_set_point AENC (N.@"m") cca_pred with "Haenc")
+  as "[#Hpred Htoken]".
+iMod (inv_alloc tokenN _ (seal_pred_rel_token_point AENC (N.@"m")) with "Htoken")
+  as "#Htok".
+iIntros "!> !> %c %c' #Hc".
+by iApply (rel_alice_guess_wrapped with "Hctx Hpred Htok Hc").
+Qed.
